cleanup

examples/NSL_with_properties/DY.NSLP.Invariants.Proofs.fst
@@ -26,8 +26,7 @@ val send_msg1_invariant:
   alice:principal -> bob:principal -> alice_public_keys_sid:state_id ->
   tr:trace ->
   Lemma
-  ( requires trace_invariant tr
-  )
+  (requires trace_invariant tr)
   (ensures (
     let (_ , tr_out) = send_msg1 alice bob alice_public_keys_sid tr in
     trace_invariant tr_out
@@ -67,11 +66,8 @@ val decode_msg1_proof:
     (ensures (
       match decode_msg1 bob bob_private_keys_sid msg tr with
       | (None, _) -> True
-      | (Some msg1, _) -> (
-          let n_a = msg1.n_a in
-          let alice = msg1.alice in
+      | (Some {alice; n_a}, _) ->
           is_knowable_by (nonce_label alice bob) tr n_a
-        )
     ))
 let decode_msg1_proof bob bob_private_keys_sid msg tr =
       match decode_msg1 bob bob_private_keys_sid msg tr with
@@ -81,7 +77,7 @@ let decode_msg1_proof bob bob_private_keys_sid msg tr =
           let plain = serialize message_t (Msg1 msg1) in
           parse_wf_lemma message_t (bytes_invariant tr) plain;
           FStar.Classical.move_requires (parse_wf_lemma message_t (is_publishable tr)) plain
-  )
+      )
 
 val receive_msg1_and_send_msg2_invariant:
   bob:principal -> 
@@ -89,8 +85,7 @@ val receive_msg1_and_send_msg2_invariant:
   msg_ts:timestamp -> 
   tr:trace ->
   Lemma
-  ( requires trace_invariant tr
-  )
+  (requires trace_invariant tr)
   (ensures (
     let (_ , tr_out) = receive_msg1_and_send_msg2 bob bob_private_keys_sid bob_public_keys_sid msg_ts tr in
     trace_invariant tr_out
@@ -101,21 +96,28 @@ let receive_msg1_and_send_msg2_invariant bob bob_private_keys_sid bob_public_key
   | (Some msg, _) -> (
       match decode_msg1 bob bob_private_keys_sid msg tr with
       | (None, _) -> ()
-      | (Some {alice; n_a}, _) -> (
+      | (Some msg1, _) -> (
+          let alice = msg1.alice in
+          let n_a = msg1.n_a in
+          
           let (n_b, tr_rand) = gen_rand_labeled (nonce_label alice bob) tr in
           assert(trace_invariant tr_rand);
+          
           let (_, tr_ev) = trigger_event bob (Responding1 {alice; bob; n_a; n_b}) tr_rand in
           assert(trace_invariant tr_ev);
+          
           let msg2 = Msg2 {bob; n_a; n_b} in
           match pke_enc_for bob alice bob_public_keys_sid key_tag msg2 tr_ev with
           | (None, _) -> ()
           | (Some msg2_encrypted, tr_msg2) ->(
               assert(trace_invariant tr_msg2);
+              
               let (msg2_ts, tr_msg2_) = send_msg msg2_encrypted tr_msg2 in
-              decode_msg1_proof bob bob_private_keys_sid msg tr;
-              serialize_wf_lemma message_t (is_knowable_by (nonce_label alice bob) tr_rand) msg2;
-              pke_enc_for_is_publishable tr_ev bob alice bob_public_keys_sid key_tag msg2;
+                decode_msg1_proof bob bob_private_keys_sid msg tr;
+                serialize_wf_lemma message_t (is_knowable_by (nonce_label alice bob) tr_rand) msg2;
+                pke_enc_for_is_publishable tr_ev bob alice bob_public_keys_sid key_tag msg2;
               assert(trace_invariant tr_msg2_);
+              
               let state = SentMsg2 {alice; n_a; n_b} in
               let (sess_id, tr_sess) = start_new_session bob state tr_msg2_ in
               assert(trace_invariant tr_sess)
@@ -142,22 +144,19 @@ val decode_msg2_proof:
   msg:bytes ->
   tr:trace ->
   Lemma
-    (requires 
-       trace_invariant tr /\
-       bytes_invariant tr msg
-    )
-    (ensures (
-      match decode_msg2 alice alice_private_keys_sid msg tr with
-      | (None, _) -> True
-      | (Some msg2, _) -> (
-          let bob = msg2.bob in
-          let n_a = msg2.n_a in
-          let n_b = msg2.n_b in
-          is_knowable_by (nonce_label alice bob) tr n_b /\
-          ( is_publishable tr n_a \/
-            event_triggered tr bob (Responding1 {alice; bob; n_a; n_b}))
-       )
-    ))
+  (requires 
+     trace_invariant tr /\
+     bytes_invariant tr msg
+  )
+  (ensures (
+    match decode_msg2 alice alice_private_keys_sid msg tr with
+    | (None, _) -> True
+    | (Some {bob; n_a; n_b}, _) -> (
+        is_knowable_by (nonce_label alice bob) tr n_b /\
+        ( is_publishable tr n_a \/
+          event_triggered tr bob (Responding1 {alice; bob; n_a; n_b}))
+     )
+  ))
 let decode_msg2_proof alice alice_private_keys_sid msg tr =
   match decode_msg2 alice alice_private_keys_sid msg tr with
   | (None, _) -> ()
@@ -175,8 +174,7 @@ val receive_msg2_and_send_msg3_invariant:
   msg_ts:timestamp -> 
   tr:trace ->
   Lemma
-  ( requires trace_invariant tr
-  )
+  (requires trace_invariant tr)
   (ensures (
     let (_ , tr_out) = receive_msg2_and_send_msg3 alice alice_private_keys_sid alice_public_keys_sid msg_ts tr in
     trace_invariant tr_out
@@ -201,17 +199,20 @@ let receive_msg2_and_send_msg3_invariant alice alice_private_keys_sid alice_publ
             | (None, _) -> ()
             | (Some (sid, st), _ ) -> (
                  let ((), tr_ev) = trigger_event alice (Responding2 {alice; bob; n_a; n_b}) tr in
-                 decode_msg2_proof alice alice_private_keys_sid msg2_ tr;
+                   decode_msg2_proof alice alice_private_keys_sid msg2_ tr;
                  assert(trace_invariant tr_ev);
+                 
                  let msg3 = Msg3 {n_b} in
                  match pke_enc_for alice bob alice_public_keys_sid key_tag msg3 tr_ev with
                  | (None, _ ) -> ()
                  | (Some msg3_encrypted, tr_enc) -> (
                       assert(trace_invariant tr_enc);
+                      
                       let (_, tr_msg3) = send_msg msg3_encrypted tr_enc in
-                      serialize_wf_lemma message_t (is_knowable_by (nonce_label alice bob) tr) msg3;
-                      pke_enc_for_is_publishable tr_ev alice bob alice_public_keys_sid key_tag msg3; 
+                        serialize_wf_lemma message_t (is_knowable_by (nonce_label alice bob) tr) msg3;
+                        pke_enc_for_is_publishable tr_ev alice bob alice_public_keys_sid key_tag msg3; 
                       assert(trace_invariant tr_msg3);
+                      
                       let state = SentMsg3 {bob; n_a; n_b} in
                       let ((), tr_st) = set_state alice sid state tr_msg3 in
                       assert(trace_invariant tr_st)
@@ -241,22 +242,21 @@ val decode_msg3_proof:
   msg:bytes ->
   tr:trace ->
   Lemma
-    (requires 
-       trace_invariant tr /\
-       bytes_invariant tr msg
-    )
-    (ensures (
-      match decode_msg3 bob bob_private_keys_sid msg tr with
-      | (None, _) -> True
-      | (Some msg3, _) -> (
-           let n_b = msg3.n_b in
-           is_publishable tr n_b \/ (
-              exists alice n_a.
-                  get_label tr n_b `can_flow tr` (nonce_label alice bob) /\
-                  event_triggered tr alice (Responding2 {alice; bob; n_a; n_b})
-           )
-        )
-    ))
+  (requires 
+     trace_invariant tr /\
+     bytes_invariant tr msg
+  )
+  (ensures (
+    match decode_msg3 bob bob_private_keys_sid msg tr with
+    | (None, _) -> True
+    | (Some {n_b}, _) -> (
+         is_publishable tr n_b \/ (
+            exists alice n_a.
+                get_label tr n_b `can_flow tr` (nonce_label alice bob) /\
+                event_triggered tr alice (Responding2 {alice; bob; n_a; n_b})
+         )
+      )
+  ))
 let decode_msg3_proof bob bob_private_keys_sid msg tr = 
   match decode_msg3 bob bob_private_keys_sid msg tr with
   | (None, _) -> ()
@@ -273,13 +273,11 @@ val receive_msg3_invariant:
   msg_ts:timestamp ->
   tr:trace ->
   Lemma
-    (requires
-      trace_invariant tr
-    )
-    (ensures (
-      let (_, tr_out) = receive_msg3 bob bob_private_keys_sid msg_ts tr in
-      trace_invariant tr_out
-    ))
+  (requires trace_invariant tr)
+  (ensures (
+    let (_, tr_out) = receive_msg3 bob bob_private_keys_sid msg_ts tr in
+    trace_invariant tr_out
+  ))
 let receive_msg3_invariant bob bob_private_keys_sid msg_ts tr = 
   match recv_msg msg_ts tr with
   | (None, _ ) -> ()
@@ -299,8 +297,9 @@ let receive_msg3_invariant bob bob_private_keys_sid msg_ts tr =
                  let n_a = (SentMsg2?.sentmsg2 st).n_a in
 
                  let (_, tr_ev) = trigger_event bob (Finishing {alice; bob; n_a; n_b}) tr in
-                 decode_msg3_proof bob bob_private_keys_sid msg3_ tr;
+                   decode_msg3_proof bob bob_private_keys_sid msg3_ tr;
                  assert(trace_invariant tr_ev);
+                 
                  let (_, tr_st) = set_state bob sid (ReceivedMsg3 {alice; n_a; n_b}) tr_ev in
                  assert(trace_invariant tr_st)
             )
