examples/NSL/DY.NSL.Run.Printing.fst
@@ -34,5 +34,5 @@ val get_trace_to_string_printers: trace_to_string_printers
 let get_trace_to_string_printers  = 
   trace_to_string_printers_builder 
     message_to_string
-    ((local_state_state.tag, state_to_string) :: default_state_to_string)
+    ((local_state_state_t.tag, state_to_string) :: default_state_to_string)
     []
