examples/NSL_with_properties/DY.NSLP.Run.Printing.fst
@@ -9,9 +9,8 @@ open DY.Simplified
 open DY.NSLP.Data
 
 /// Helper functions for trace printing.
-/// Here we define how our abstract message and state types
+/// Here we define how our abstract message, state and event types
 /// should be printed.
-
 
 val message_to_string: bytes -> option string
 let message_to_string b =
@@ -19,7 +18,6 @@ let message_to_string b =
   | Msg1 m -> Some (Printf.sprintf "Msg1 [name = (%s), n_a = (%s)]" (m.alice) (bytes_to_string m.n_a))
   | Msg2 m -> Some (Printf.sprintf "Msg2 [name = (%s), n_a = (%s), n_b = (%s)]" (m.bob) (bytes_to_string m.n_a) (bytes_to_string m.n_b))
   | Msg3 m -> Some (Printf.sprintf "Msg3 [n_b = (%s)]" (bytes_to_string m.n_b))
-
 
 val state_to_string: bytes -> option string
 let state_to_string b =
@@ -38,10 +36,9 @@ let event_to_string b =
     | Finishing {alice; bob; n_a; n_b} -> Some (Printf.sprintf "Finishing [bob = (%s), n_a = (%s), n_b = (%s), with = (%s)]" bob (bytes_to_string n_a) (bytes_to_string n_b) alice)
 
 
-
 val get_trace_to_string_printers: trace_to_string_printers
 let get_trace_to_string_printers  = 
   trace_to_string_printers_builder 
     message_to_string
-    ((local_state_state.tag, state_to_string) :: default_state_to_string)
+    ((local_state_state_t.tag, state_to_string) :: default_state_to_string)
     [(event_event_t.tag, event_to_string)]
